Complete Lab 2 Dafny

Lab2/CircularMemory.dfy
@@ -5,67 +5,113 @@
 // The first task is to complete this constructor by supplying sufficient pre-condition.
 class CircularMemory
 {
-  var cells : array<int>
-  var read_position : int
-  var write_position : int
-  var isFlipped : bool
+    var cells : array<int>
+    var read_position : int
+    var write_position : int
+    var isFlipped : bool
 
-  constructor Init(cap : int)
-  requires cap >= 0
-  {
-    cells := new int[cap];
-    read_position, write_position := 0, 0;
-    isFlipped := false;
-  }
+    constructor Init(cap : int)
+    requires cap >= 0
+    {
+        cells := new int[cap];
+        read_position, write_position := 0, 0;
+        isFlipped := false;
+    }
 
     // Valid is the class invariant we would like to maintain
-  // for any CircularMemory at any moment of its lifetime
-  predicate Valid()
+    // for any CircularMemory at any moment of its lifetime
+    predicate Valid()
     reads this
-  {
+    {
+        // Pointer positioning in array 
+        var validArrayIndexes := read_position >= 0 
+        && write_position >= 0 
+        && read_position < cells.Length 
+        && write_position < cells.Length;
 
-    // Pointer positioning in array 
-    var validArrayIndexes := read_position >= 0 
-    && write_position >= 0 
-    && read_position < cells.Length 
-    && write_position < cells.Length;
+        // Validate isFlipped with respect to read/write position 
+        var correctPointerPos := (
+            if isFlipped 
+            then read_position >= write_position
+            else write_position >= read_position
+        );
 
-    // Validate isFlipped with respect to read/write position 
-    var correctPointerPos := (
-          if isFlipped then read_position > write_position
-          else write_position >= read_position
-    );
+        validArrayIndexes && correctPointerPos
+    }
 
-  
-  validArrayIndexes && correctPointerPos
+    // A predicate indicating no more Read available
+    predicate isEmpty()
+    requires Valid()
+        reads this
+    {
+        read_position == write_position && !isFlipped
+    }
 
-  }
+    // A predicate indicating no more Write should be allowed
+    predicate isFull()
+    requires Valid()
+        reads this
+    {
+        write_position == read_position && isFlipped
+    }
 
-  // A predicate indicating no more Read available
-  predicate isEmpty()
-  requires Valid()
-    reads this
-  {
-    read_position == write_position 
-  }
 
-  //A predicate indicating no more Write should be allowed
-  predicate isFull()
-  requires Valid()
-    reads this
-  {
-  
-  if isFlipped then 
-    write_position == read_position - 1
-  else 
-    write_position == cells.Length -1 && read_position == 0   
-    
-  }
+    method Read() returns (isSuccess : bool, content : int)
+        modifies this
+        requires Valid()
+        ensures  Valid()
+        ensures  isSuccess ==> (
+            var prev := if read_position - 1 < 0 then cells.Length - 1 else read_position - 1;
+
+            content == cells[prev]
+        )
+        ensures !isSuccess ==> isEmpty()
+    {
+        if (isEmpty())
+        {
+            return false, 0;
+        }
+        
+        var read_val := cells[read_position];
+
+        read_position := read_position + 1;
+        if (read_position == cells.Length)
+        {
+            read_position := 0;
+            isFlipped := false;
+        }
+
+        return true, read_val;
+    }
+
+    method Write(input : int) returns (isSuccess : bool)
+        modifies this
+        modifies cells
+        requires Valid()
+        ensures  Valid()
+        ensures  isSuccess ==> (
+            var prev := if write_position - 1 < 0 then cells.Length - 1 else write_position - 1;
+
+            input == cells[prev]
+        )
+        ensures !isSuccess ==> isFull()
+    {
+        if (isFull())
+        {
+            return false;
+        }
+
+        cells[write_position] := input;
+        
+        write_position := write_position + 1;
+        if (write_position == cells.Length)
+        {
+            write_position := 0;
+            isFlipped := true;
+        }
+
+        return true;
+    }
+
+
 }
-
-
-
-
-
-  
-
